leetcode/0101-symmetric-tree.dfy
@@ -1,10 +1,11 @@
 // Author: Shaobo He
 include "../lib/adt/BinaryTree.dfy"
+include "0226-invert-binary-tree.dfy"
 
 import opened BinaryTree
 
 method isMirror?<T(==)>(t1: Tree<T>, t2: Tree<T>) returns(r: bool)
-ensures r <==> equal?(t1, mirror(t2));
+ensures r <==> Equal?(t1, Mirror(t2));
 {
     if (t1.Nil? && t2.Nil?) {
         return true;
@@ -18,7 +19,7 @@ ensures r <==> equal?(t1, mirror(t2));
 }
 
 method isSymmetric<T(==)>(root: Tree<T>) returns(r: bool)
-ensures r <==> equal?(root, mirror(root));
+ensures r <==> Equal?(root, Mirror(root));
 {
     r := isMirror?(root, root);
 }
